candle/prover/compute/computePmatchScript.sml
@@ -1,0 +1,62 @@
+(*
+  Pmatch definitions for functions in computeScript.sml.
+ *)
+
+open preamble computeTheory;
+local open patternMatchesLib in end;
+
+val _ = new_theory "computePmatch";
+
+val _ = numLib.prefer_num ();
+
+val _ = patternMatchesLib.ENABLE_PMATCH_CASES ();
+
+Theorem dest_num_PMATCH:
+  ∀tm.
+    dest_num tm =
+      case tm of
+        Const n t => if tm = _0 then SOME 0 else NONE
+      | Comb (Const nm t) r =>
+          (case dest_num r of
+          | NONE => NONE
+          | SOME n => if Const nm t = _BIT0_TM then SOME (2 * n)
+                      else if Const nm t = _BIT1_TM then SOME (2 * n + 1)
+                      else NONE)
+      | _ => NONE
+Proof
+  CONV_TAC (DEPTH_CONV patternMatchesLib.PMATCH_ELIM_CONV)
+  \\ rw [Once dest_num_def]
+QED
+
+Theorem dest_numeral_PMATCH:
+  ∀tm.
+    dest_numeral tm =
+      case tm of
+        Comb (Const n t) r =>
+          if Const n t = _NUMERAL_TM then
+            case dest_num r of
+            | NONE => raise_Failure «dest_numeral»
+            | SOME n => st_ex_return n
+          else
+            raise_Failure «dest_numeral»
+      | _ => raise_Failure «dest_numeral»
+Proof
+  CONV_TAC (DEPTH_CONV patternMatchesLib.PMATCH_ELIM_CONV)
+  \\ rw [Once dest_numeral_def]
+QED
+
+Theorem dest_binary_PMATCH:
+  ∀tm' tm.
+    dest_binary tm' tm =
+      case tm of
+        Comb (Comb (Const n t) l) r =>
+          if tm' = Const n t then st_ex_return (l, r)
+          else raise_Failure «dest_binary»
+      | _ => raise_Failure «dest_binary»
+Proof
+  CONV_TAC (DEPTH_CONV patternMatchesLib.PMATCH_ELIM_CONV)
+  \\ rw [Once dest_binary_def]
+QED
+
+val _ = export_theory ();
+
