candle/prover/compute/README.md
@@ -1,5 +1,8 @@
 A verified Candle compute primitive.
 
+[computePmatchScript.sml](computePmatchScript.sml):
+Pmatch definitions for functions in computeScript.sml.
+
 [computeScript.sml](computeScript.sml):
 Implementation of the compute primitive.
 
